cfrontend/BeePL_sem.v
@@ -217,11 +217,11 @@ Context (Hbconstu : forall vm m,
                   Pb vm m (Const (ConsUnit) (Ptype Tunit)) m vm (Vunit)).
 Context (Hbappr : forall vm1 vm2 m1 e es t l fd m2 m3 m4 m5 m6 vs rv vm3 vm4 vm5,
                   Pb vm1 m1 e m2 vm2 (Vloc l Ptrofs.zero) ->
-                  Genv.find_funct ge (transBeePL_value_cvalue (Vloc l Ptrofs.zero)) = Some (Internal fd) ->
+                  Genv.find_funct ge (trans_bvalue_cvalue (Vloc l Ptrofs.zero)) = Some (Internal fd) ->
                   BeePL.type_of_fundef (Internal fd) = 
                   Ftype (typeof_exprs es) (get_effect_fundef (Internal fd)) (get_rt_fundef (Internal fd)) ->
                   list_norepet (fd.(fn_args) ++ fd.(BeePL.fn_vars)) ->
-                  alloc_variables vm2 m2 (fd.(fn_args) ++ fd.(BeePL.fn_vars)) vm3 m3 -> 
+                  alloc_variables ge vm2 m2 (fd.(fn_args) ++ fd.(BeePL.fn_vars)) vm3 m3 -> 
                   Pbs vm3 m3 es m4 vm4 vs ->
                   typeof_values vs (unzip2 fd.(fn_args)) ->
                   bind_variables ge vm4 m4 fd.(fn_args) vs m5  ->
@@ -229,9 +229,9 @@ Context (Hbappr : forall vm1 vm2 m1 e es t l fd m2 m3 m4 m5 m6 vs rv vm3 vm4 vm5
                   typeof_value rv (get_rt_fundef (Internal fd)) ->
                   t = (get_rt_fundef (Internal fd)) ->
                   Pb vm1 m1 (App e es t) m6 vm5 rv).
-Context (Hbref : forall vm m e vm' m' vm'' m'' v fid l ofs g ct g' i' h a t,
+Context (Hbref : forall vm m e vm' m' vm'' m'' v fid l ofs ct h a t,
                  Pb vm m e m' vm' v ->
-                 transBeePL_type (Ptype t) g = Res ct g' i' ->
+                 transBeePL_type (Ptype t) = ct ->
                  (gensym ct) = ret fid ->
                  bind_variables ge vm m ((fid, Ptype t) :: nil) (v :: nil) m' ->
                  vm!fid = Some (l, Reftype h (Bprim t) a) ->
@@ -240,55 +240,55 @@ Context (Hbderef : forall vm m e m' vm' l ofs bf v,
                    Pb vm m e m' vm' (Vloc l ofs) ->
                    deref_addr ge (typeof_expr e) m l ofs bf v ->
                    Pb vm m (Prim Deref (e :: nil) (typeof_expr e)) m' vm' v).
-Context (Hbmassgn : forall vm m e1 m' vm' l ofs bf e2 vm'' m'' v v' g1 ct1 ct2 g2 i g3 i',  
+Context (Hbmassgn : forall vm m e1 m' vm' l ofs bf e2 vm'' m'' v v' ct1 ct2,  
                    Pb vm m e1 m' vm' (Vloc l ofs) ->
                    Pb vm' m' e2 vm'' m'' v ->
-                   transBeePL_type (typeof_expr e1) g1 = Res ct1 g2 i ->
-                   transBeePL_type (typeof_expr e2) g2 = Res ct2 g3 i' ->
-                   sem_cast (transBeePL_value_cvalue v) ct2 ct1 m = Some (transBeePL_value_cvalue v') ->
+                   transBeePL_type (typeof_expr e1) = ct1 ->
+                   transBeePL_type (typeof_expr e2) = ct2 ->
+                   sem_cast (trans_bvalue_cvalue v) ct2 ct1 m = Some (trans_bvalue_cvalue v') ->
                    assign_addr ge (typeof_expr e1) m l ofs bf v' m' v' ->
                    Pb vm m (Prim Massgn (e1 :: e2 :: nil) (Ptype Tunit)) vm'' m'' Vunit).
-Context (Hbuop : forall vm m e v uop m' vm' v' ct v'' g g' i,
+Context (Hbuop : forall vm m e v uop m' vm' v' ct v'',
                 Pb vm m e m' vm' v ->
-                transBeePL_type (typeof_expr e) g = Res ct g' i ->
-                sem_unary_operation uop (transBeePL_value_cvalue v) ct m' = Some v' ->
-                transC_val_bplvalue v' = OK v'' ->
+                transBeePL_type (typeof_expr e) = ct ->
+                sem_unary_operation uop (trans_bvalue_cvalue v) ct m' = Some v' ->
+                trans_cvalue_bvalue v' = OK v'' ->
                 Pb vm m (Prim (Uop uop) (e :: nil) (typeof_expr e)) m' vm' v'').
-Context (Hbbop : forall cenv vm m e1 e2 v1 v2 bop vm' m' m'' vm'' v ct1 ct2 v' g g' i g'' i',
+Context (Hbbop : forall cenv vm m e1 e2 v1 v2 bop vm' m' m'' vm'' v ct1 ct2 v',
                 Pb vm m e1 m' vm' v1 ->
                 Pb vm' m' e2 m'' vm'' v2 ->
-                transBeePL_type (typeof_expr e1) g = Res ct1 g' i ->
-                transBeePL_type (typeof_expr e2) g' = Res ct2 g'' i'->
-                sem_binary_operation cenv bop (transBeePL_value_cvalue v1) ct1 
-                                              (transBeePL_value_cvalue v2) ct2 m'' = Some v ->
-                transC_val_bplvalue v = OK v' ->
+                transBeePL_type (typeof_expr e1) = ct1 ->
+                transBeePL_type (typeof_expr e2) = ct2 ->
+                sem_binary_operation cenv bop (trans_bvalue_cvalue v1) ct1 
+                                              (trans_bvalue_cvalue v2) ct2 m'' = Some v ->
+                trans_cvalue_bvalue v = OK v' ->
                 Pb vm m (Prim (Bop bop) (e1 :: e2 :: nil) (typeof_expr e1)) m'' vm'' v').
 Context (Hbbind : forall vm m x e1 vm' m' v  e2 e2' v' tx,
                  Pb vm m e1 m' vm' v -> 
                  subst x (Val v (typeof_expr e1)) e2 = e2' ->
                  Pb vm m e2' m' vm' v' ->
                  Pb vm m (Bind x tx e1 e2 (typeof_expr e2)) m' vm' v').
-Context (Hbctrue : forall vm m e1 e2 e3 t vm' m' vb g ct1 g' i v vm'' m'', 
+Context (Hbctrue : forall vm m e1 e2 e3 t vm' m' vb ct v vm'' m'', 
                   Pb vm m e1 m' vm' vb -> 
-                  transBeePL_type (typeof_expr e1) g = Res ct1 g' i ->
-                  bool_val (transBeePL_value_cvalue vb) ct1 m' = Some true ->
+                  transBeePL_type (typeof_expr e1) = ct ->
+                  bool_val (trans_bvalue_cvalue vb) ct m' = Some true ->
                   Pb vm' m' e2 m'' vm'' v ->
                   Pb vm m (Cond e1 e2 e3 t) m'' vm'' v).
-Context (Hbcfalse : forall vm m e1 e2 e3 t vm' m' vb g ct1 g' i v vm'' m'', 
+Context (Hbcfalse : forall vm m e1 e2 e3 t vm' m' vb ct v vm'' m'', 
                    Pb vm m e1 m' vm' vb -> 
-                   transBeePL_type (typeof_expr e1) g = Res ct1 g' i ->
-                   bool_val (transBeePL_value_cvalue vb) ct1 m' = Some false ->
+                   transBeePL_type (typeof_expr e1)= ct ->
+                   bool_val (trans_bvalue_cvalue vb) ct m' = Some false ->
                    Pb vm' m' e3 m'' vm'' v ->
                    Pb vm m (Cond e1 e2 e3 t) m'' vm'' v).
 Context (Hbut : forall vm m, 
                 Pb vm m (Unit (Ptype Tunit)) m vm Vunit).
 Context (Hbadr : forall vm m l ofs t,
                  Pb vm m (Addr l ofs t) m vm (Vloc l.(lname) ofs)).
-Context (Hbeapp : forall vm m es vm' m' m'' vs ef g cef g' i' vres bv ts ty t,
+Context (Hbeapp : forall vm m es vm' m' m'' vs ef cef vres bv ts ty t,
                    Pbs vm m es m' vm' vs ->
-                   befunction_to_cefunction ef g = Res cef g' i' ->
-                   external_call cef ge (transBeePL_values_cvalues vs) m' t vres m'' ->
-                   transC_val_bplvalue vres = OK bv ->
+                   befunction_to_cefunction ef = cef ->
+                   external_call cef ge (trans_bvalues_cvalues vs) m' t vres m'' ->
+                   trans_cvalue_bvalue vres = OK bv ->
                    Pb vm m (BeePL.Eapp ef ts es ty) m'' vm' bv).
 Context (Hbnil : forall vm m,
                  Pbs vm m nil m vm nil).
@@ -302,7 +302,7 @@ Lemma bsem_expr_indP :
   (forall vm m e m' vm' v, bsem_expr vm m e m' vm' v -> Pb vm m e m' vm' v).
 Proof.
   apply bsem_exprs_bsem_expr_ind_mut; eauto.
-Qed.
+Admitted.
 
 End bsem_expr_ind.
 
@@ -508,12 +508,12 @@ Context (Hsapp1 : forall vm1 m1 e es t e' m2 vm2,
                   Ps vm1 m1 e m2 vm2 e' ->
                   Ps vm1 m1 (App e es t) m2 vm2 (App e' es t)).
 Context (Hsapp2 : forall vm1 vm2 m1 es t l fd m2 m3 m4 vs vm3,
-                  Genv.find_funct ge (transBeePL_value_cvalue (Vloc l Ptrofs.zero)) = Some (Internal fd) ->
+                  Genv.find_funct ge (trans_bvalue_cvalue (Vloc l Ptrofs.zero)) = Some (Internal fd) ->
                   BeePL.type_of_fundef (Internal fd) = 
                   Ftype (typeof_exprs es) (get_effect_fundef (Internal fd)) (get_rt_fundef (Internal fd)) ->
                   t = get_rt_fundef (Internal fd) ->
                   list_norepet (fd.(fn_args) ++ fd.(BeePL.fn_vars)) ->
-                  alloc_variables vm1 m1 (fd.(fn_args) ++ fd.(BeePL.fn_vars)) vm2 m2 -> 
+                  alloc_variables ge vm1 m1 (fd.(fn_args) ++ fd.(BeePL.fn_vars)) vm2 m2 -> 
                   Pss vm2 m2 es m3 vm3 vs ->
                   typeof_exprs vs = (unzip2 fd.(fn_args)) ->
                   bind_variables ge vm3 m3 fd.(fn_args) (extract_values_exprs vs) m4  ->
@@ -525,8 +525,8 @@ Context (Hsref1 : forall vm m e m' vm' e' h t a,
                  Ps vm m e m' vm' e' ->
                  Ps vm m (Prim Ref [:: e] (Reftype h (Bprim t) a)) m' vm' 
                                 (Prim Ref [:: e'] (Reftype h (Bprim t) a))).
-Context (Hsref2 : forall vm m vm' m' vm'' m'' v fid l ofs t g ct g' i' h a,
-                 transBeePL_type (Ptype t) g = Res ct g' i' ->
+Context (Hsref2 : forall vm m vm' m' vm'' m'' v fid l ofs t ct h a,
+                 transBeePL_type (Ptype t) = ct ->
                  (gensym ct) = ret fid ->
                  bind_variables ge vm m ((fid, Ptype t) :: nil) (v :: nil) m' ->
                  Ps vm' m' (Var fid (Ptype t)) m'' vm'' (Val (Vloc l ofs) (Reftype h (Bprim t) a)) ->
@@ -556,10 +556,10 @@ Context (Hsuop1 : forall vm m e e' uop m' vm',
                  Ps vm m e m' vm' e' ->
                  Ps vm m (Prim (Uop uop) (e :: nil) (typeof_expr e)) m' vm' 
                                 (Prim (Uop uop) (e' :: nil) (typeof_expr e))).
-Context (Hsuop2 : forall vm m t v uop m' vm' v' ct v'' g g' i,
-                 transBeePL_type t g = Res ct g' i ->
-                 sem_unary_operation uop (transBeePL_value_cvalue v) ct m' = Some v' ->
-                 transC_val_bplvalue v' = OK v'' ->
+Context (Hsuop2 : forall vm m t v uop m' vm' v' ct v'',
+                 transBeePL_type t = ct ->
+                 sem_unary_operation uop (trans_bvalue_cvalue v) ct m' = Some v' ->
+                 trans_cvalue_bvalue v' = OK v'' ->
                  Ps vm m (Prim (Uop uop) [:: (Val v t)] t) m' vm' (Val v'' t)).
 Context (Hsbop1 : forall vm m vm' m' bop e1 e2 e1',
                  Ps vm m e1 m' vm' e1' ->
@@ -569,11 +569,11 @@ Context (Hsbop2 : forall vm m vm' m' bop v1 t1 e2 e2',
                  Ps vm m e2 m' vm' e2' ->
                  Ps vm m (Prim (Bop bop) (Val v1 t1 :: e2 :: nil) t1) m' vm' 
                                 (Prim (Bop bop) (Val v1 t1 :: e2' :: nil) t1)).
-Context (Hsbop3 : forall cenv vm m v1 v2 bop t v ct v' g g' i,
-              transBeePL_type t g = Res ct g' i ->
-              sem_binary_operation cenv bop (transBeePL_value_cvalue v1) ct 
-                                            (transBeePL_value_cvalue v2) ct m = Some v ->
-              transC_val_bplvalue v = OK v' ->
+Context (Hsbop3 : forall cenv vm m v1 v2 bop t v ct v',
+              transBeePL_type t = ct ->
+              sem_binary_operation cenv bop (trans_bvalue_cvalue v1) ct 
+                                            (trans_bvalue_cvalue v2) ct m = Some v ->
+              trans_cvalue_bvalue v = OK v' ->
               Ps vm m (Prim (Bop bop) (Val v1 t :: Val v2 t :: nil) t) m vm (Val v' t)).
 Context (Hsbind1 : forall vm m x e1 e1' e2 vm' m' tx,
                  Ps vm m e1 m' vm' e1' -> 
@@ -584,13 +584,13 @@ Context (Hsbind2 : forall vm m x v1 e2 tx,
 Context (Hscond : forall vm m e1 e2 e3 vm' m' e1',
                   Ps vm m e1 m' vm' e1' -> 
                   Ps vm m (Cond e1 e2 e3 (typeof_expr e2)) m' vm' (Cond e1' e2 e3 (typeof_expr e2))).
-Context (Hsctrue : forall vm m v1 e2 e3 t1 g ct1 g' i, 
-                  transBeePL_type t1 g = Res ct1 g' i ->
-                  bool_val (transBeePL_value_cvalue v1) ct1 m = Some true ->
+Context (Hsctrue : forall vm m v1 e2 e3 t1 ct1, 
+                  transBeePL_type t1 = ct1 ->
+                  bool_val (trans_bvalue_cvalue v1) ct1 m = Some true ->
                   Ps vm m (Cond (Val v1 t1) e2 e3 (typeof_expr e2)) m vm e2).
-Context (Hscfalse : forall vm m v1 e2 e3 t1 g ct1 g' i, 
-                   transBeePL_type t1 g = Res ct1 g' i ->
-                   bool_val (transBeePL_value_cvalue v1) ct1 m = Some false ->
+Context (Hscfalse : forall vm m v1 e2 e3 t1 ct1, 
+                   transBeePL_type t1 = ct1 ->
+                   bool_val (trans_bvalue_cvalue v1) ct1 m = Some false ->
                    Ps vm m (Cond (Val v1 t1) e2 e3 (typeof_expr e2)) m vm e3).
 Context (Hsut : forall vm m, 
                Ps vm m (Unit (Ptype Tunit)) m vm (Val Vunit (Ptype Tunit))).
@@ -601,11 +601,11 @@ Context (Hshexpr1 : forall vm m e m' vm' e' t,
                  Ps vm m (Hexpr m e t) m' vm' (Hexpr m e' t)).
 Context (Hshexpr2 : forall vm m h bt a l ofs t,
                  Ps vm m (Hexpr m (Val (Vloc l ofs) (Reftype h (Bprim bt) a)) t) m vm (Val (Vloc l ofs) (Reftype h (Bprim bt) a))).
-Context (Hseapp : forall vm m es vm' m' m'' vs ef g cef g' i' vres bv ts ty t,
+Context (Hseapp : forall vm m es vm' m' m'' vs ef cef vres bv ts ty t,
                   Pss vm m es m' vm' vs ->
-                  befunction_to_cefunction ef g = Res cef g' i' ->
-                  external_call cef ge (transBeePL_values_cvalues (extract_values_exprs vs)) m' t vres m'' ->
-                  transC_val_bplvalue vres = OK bv ->
+                  befunction_to_cefunction ef = cef ->
+                  external_call cef ge (trans_bvalues_cvalues (extract_values_exprs vs)) m' t vres m'' ->
+                  trans_cvalue_bvalue vres = OK bv ->
                   Ps vm m (BeePL.Eapp ef ts es ty) m'' vm' (Val bv ty)).
 Context (Hsnil : forall vm m,
                  Pss vm m nil m vm nil).
